@@ -64,3 +64,6 @@ import MachCSL.ByteWord
 import MachCSL.WpSmodeMint
 import MachCSL.WpSmodeAlu2
 import MachCSL.WpSmodeAlu4
+import MachCSL.KCtxMove
+import MachCSL.SwtchCtx
+import MachCSL.WpSmodeSwtch
